Move all parameters & axioms to 'Parameters.v'

Structures/Forests.v
@@ -4,7 +4,7 @@ Require Import Eqdep.
 From fcsl
 Require Import pred prelude ordtype pcm finmap unionmap heap.
 From Toychain
-Require Import SeqFacts Chains Blocks.
+Require Import SeqFacts Chains Parameters.
 Set Implicit Arguments.
 Unset Strict Implicit.
 Unset Printing Implicit Defensive.
@@ -12,92 +12,10 @@ Unset Printing Implicit Defensive.
 (* A formalization of a block forests *)
 (* TODO: Go through this file and put the lemmas in a sensible order. *)
 
-(************************************************************)
-(******************* <parameters> ***************************)
-(************************************************************)
-
-Parameter Timestamp : Type.
-Parameter Hash : ordType.
-Parameter VProof : eqType.
-Parameter Transaction : eqType.
-Parameter Address : finType.
-
-Definition block := @Block Hash Transaction VProof.
-
-Parameter GenesisBlock : block.
-
-Definition Blockchain := seq block.
-
-(* In fact, it's a forest, as it also keeps orphan blocks *)
-Definition BlockTree := union_map Hash block.
-
-(* Transaction pools *)
-Definition TxPool := seq Transaction.
-
-Parameter hashT : Transaction -> Hash.
-Parameter hashB : block -> Hash.
-Parameter genProof : Address -> Blockchain -> TxPool -> Timestamp -> option (TxPool * VProof).
-Parameter VAF : VProof -> Blockchain -> TxPool -> bool.
-Parameter FCR : Blockchain -> Blockchain -> bool.
-
-(* Transaction is valid and consistent with the given chain *)
-Parameter txValid : Transaction -> Blockchain -> bool.
-Parameter tpExtend : TxPool -> BlockTree -> Transaction -> TxPool.
-
-(************************************************************)
-(********************* </parameters> ************************)
-(************************************************************)
-
-Notation "A > B" := (FCR A B).
-Notation "A >= B" := (A = B \/ A > B).
 Notation "# b" := (hashB b) (at level 20).
 
 Definition bcLast (bc : Blockchain) := last GenesisBlock bc.
 
-Definition subchain (bc1 bc2 : Blockchain) := exists p q, bc2 = p ++ bc1 ++ q.
-
-(************************************************************)
-(*********************** <axioms> ***************************)
-(************************************************************)
-
-(* 2.  Transaction validation *)
-
-Axiom txValid_nil : forall t, txValid t [::].
-
-(* 3.  Hashes *)
-
-(* Axiom hashB_inj : injective hashB. *)
-
-(* 4.  VAF *)
-
-Axiom VAF_init : VAF (proof GenesisBlock) [::] (txs GenesisBlock).
-
-Axiom VAF_GB_first :
-  forall bc, VAF (proof GenesisBlock) bc (txs GenesisBlock) -> bc = [::].
-
-(* 2. FCR *)
-
-Axiom FCR_subchain :
-  forall bc1 bc2, subchain bc1 bc2 -> bc2 >= bc1.
-
-(* TODO: strengthen to only valid chains *)
-Axiom FCR_ext :
-  forall (bc : Blockchain) (b : block) (ext : seq block),
-    bc ++ (b :: ext) > bc.
-
-Axiom FCR_rel :
-  forall (A B : Blockchain),
-    A = B \/ A > B \/ B > A.
-
-Axiom FCR_nrefl :
-  forall (bc : Blockchain), bc > bc -> False.
-
-Axiom FCR_trans :
-  forall (A B C : Blockchain), A > B -> B > C -> A > C.
-
-(************************************************************)
-(*********************** </axioms> **************************)
-(************************************************************)
 
 Lemma FCR_trans_eq (A B C : Blockchain):
     A >= B -> B >= C -> A >= C.
