Structures/Parameters.v
@@ -1,0 +1,103 @@
+From mathcomp.ssreflect
+Require Import ssreflect ssrbool ssrnat eqtype ssrfun seq fintype path.
+From fcsl
+Require Import ordtype unionmap.
+Set Implicit Arguments.
+Unset Strict Implicit.
+Unset Printing Implicit Defensive.
+
+
+(************************************************************)
+(******************* <parameters> ***************************)
+(************************************************************)
+
+Parameter Timestamp : Type.
+Parameter Hash : ordType.
+Parameter VProof : eqType.
+Parameter Transaction : eqType.
+Parameter Address : finType.
+
+Record Block {Hash : ordType} {Transaction VProof : eqType} :=
+  mkB {
+    prevBlockHash : Hash;
+    txs : seq Transaction;
+    proof : VProof;
+  }.
+
+Definition eq_block {H : ordType} {T P : eqType} (b b' : @Block H T P) :=
+  match b, b' with
+  | mkB p t pf, mkB p' t' pf' =>
+    [&& p == p', t == t' & pf == pf']
+  end.
+
+Lemma eq_blockP {H : ordType} {T P : eqType} : Equality.axiom (@eq_block H T P).
+Proof.
+case=> p t pf; case=> p' t' pf'; rewrite /eq_block/=.
+case H2: (p == p'); [move/eqP: H2=>?; subst p'| constructor 2];
+  last by case=>?; subst p';rewrite eqxx in H2.
+case H3: (t == t'); [move/eqP: H3=>?; subst t'| constructor 2];
+  last by case=>?; subst t';rewrite eqxx in H3.
+case H4: (pf == pf'); [move/eqP: H4=>?; subst pf'| constructor 2];
+  last by case=>?; subst pf';rewrite eqxx in H4.
+by constructor 1.
+Qed.
+
+Canonical Block_eqMixin {H : ordType} {T P : eqType} :=
+  Eval hnf in EqMixin (@eq_blockP H T P).
+Canonical Block_eqType {H : ordType} {T P : eqType} :=
+  Eval hnf in EqType (@Block H T P) (@Block_eqMixin H T P).
+
+Definition block := @Block Hash Transaction VProof.
+Definition Blockchain := seq block.
+Definition subchain (bc1 bc2 : Blockchain) := exists p q, bc2 = p ++ bc1 ++ q.
+
+Definition TxPool := seq Transaction.
+(* In fact, it's a forest, as it also keeps orphan blocks *)
+Definition BlockTree := union_map Hash block.
+
+Parameter GenesisBlock : block.
+
+Parameter hashT : Transaction -> Hash.
+Parameter hashB : block -> Hash.
+
+Parameter genProof : Address -> Blockchain -> TxPool -> Timestamp -> option (TxPool * VProof).
+Parameter VAF : VProof -> Blockchain -> TxPool -> bool.
+
+Parameter FCR : Blockchain -> Blockchain -> bool.
+Notation "A > B" := (FCR A B).
+Notation "A >= B" := (A = B \/ A > B).
+
+Parameter txValid : Transaction -> Blockchain -> bool.
+Parameter tpExtend : TxPool -> BlockTree -> Transaction -> TxPool.
+
+(************************************************************)
+(*********************** <axioms> ***************************)
+(************************************************************)
+
+Axiom txValid_nil : forall t, txValid t [::].
+
+(** VAF **)
+Axiom VAF_init : VAF (proof GenesisBlock) [::] (txs GenesisBlock).
+
+Axiom VAF_GB_first :
+  forall bc, VAF (proof GenesisBlock) bc (txs GenesisBlock) -> bc = [::].
+
+
+(** FCR **)
+Axiom FCR_subchain :
+  forall bc1 bc2, subchain bc1 bc2 -> bc2 >= bc1.
+
+(* TODO: strengthen to only valid chains *)
+Axiom FCR_ext :
+  forall (bc : Blockchain) (b : block) (ext : seq block),
+    bc ++ (b :: ext) > bc.
+
+Axiom FCR_rel :
+  forall (A B : Blockchain),
+    A = B \/ A > B \/ B > A.
+
+Axiom FCR_nrefl :
+  forall (bc : Blockchain), bc > bc -> False.
+
+Axiom FCR_trans :
+  forall (A B C : Blockchain), A > B -> B > C -> A > C.
